proved that PO-numbered <-> reachable, and PO-numbering is injective.
git-svn-id: https://webdav.seas.upenn.edu/svn/sol/vol@4019 eef5ea85-cc2e-0410-bd84-0fae1f012da8

src3.0/Vellvm/Dominators/dfs.v
@@ -6,46 +6,6 @@ Require Import Metatheory.
 Require Import Program.Tactics.
 Require Import dom_libs.
 
-Import LLVMsyntax.
-
-Record Frame := mkFrame {
-  Fr_name: l;
-  Fr_scs: ls
-}.
-
-Fixpoint find_next_visit_in_scs (visited: ATree.t unit) (scs: ls) 
-  : option (l * ls) :=
-match scs with
-| nil => None
-| sc::scs' => 
-    match ATree.get sc visited with
-    | None => Some (sc, scs')
-    | _ => find_next_visit_in_scs visited scs'
-    end
-end.
-
-Record PostOrder := mkPO {
-  PO_cnt: positive;
-  PO_a2p: ATree.t positive
-}.
-
-Definition postorder_inc (po:PostOrder) (v:l) : PostOrder :=
-let '(mkPO cnt a2p) := po in
-mkPO (Psucc cnt) (ATree.set v cnt a2p).
-
-Fixpoint find_next_visit_in_stk (succs: ATree.t ls)
-  (visited: ATree.t unit) (po:PostOrder) (frs: list Frame) 
-  : l * list Frame * PostOrder + PostOrder :=
-match frs with
-| nil => inr po
-| mkFrame v scs::frs' => 
-    match find_next_visit_in_scs visited scs with
-    | Some (sc, scs') => 
-        inl (sc, mkFrame sc (succs!!!sc)::mkFrame v scs'::frs', po)
-    | None => find_next_visit_in_stk succs visited (postorder_inc po v) frs'
-    end
-end.
-
 Ltac inv_mbind_app :=
   match goal with
   | H: _ = match ?e with
@@ -58,20 +18,13 @@ Ltac inv_mbind_app :=
        end = _ |- _ => remember e as R; destruct R
   end.
 
-Lemma find_next_visit_in_scs_spec: forall visited scs sc scs'
-  (Hfind : Some (sc, scs') = find_next_visit_in_scs visited scs),
-  incl (sc::scs') scs /\ ATree.get sc visited = None.
+Lemma ATree_set_pres_nonempty: forall (n : atom) visited 
+  (Hin : visited ! n <> None) next,
+  (ATree.set next tt visited) ! n <> None.
 Proof.
-  induction scs as [|sc scs]; simpl; intros.
-    congruence.
-
-    inv_mbind_app.
-      apply IHscs in Hfind.
-      destruct_pairs.
-      split; eauto with datatypes v62.
-    
-      uniq_result.
-      split; eauto with datatypes v62.
+  intros.
+  rewrite ATree.gsspec.
+  destruct_if; congruence.
 Qed.
 
 Lemma length_le__length_lt: forall A 
@@ -89,6 +42,144 @@ Proof.
     apply remove_in_length; auto with datatypes v62.
   omega.
 Qed.
+
+(**********************************************************)
+
+Import LLVMsyntax.
+
+Record Frame := mkFrame {
+  Fr_name: l;
+  Fr_scs: ls
+}.
+
+(**********************************************************)
+
+Fixpoint find_next_visit_in_scs (visited: ATree.t unit) (scs: ls) 
+  : option (l * ls) :=
+match scs with
+| nil => None
+| sc::scs' => 
+    match ATree.get sc visited with
+    | None => Some (sc, scs')
+    | _ => find_next_visit_in_scs visited scs'
+    end
+end.
+
+Lemma find_next_visit_in_scs_spec': forall visited scs sc scs'
+  (Hfind : Some (sc, scs') = find_next_visit_in_scs visited scs),
+  exists scs0,
+    scs = scs0 ++ sc::scs' /\ 
+    (forall sc0 (Hin: In sc0 scs0), ATree.get sc0 visited <> None) /\
+    ATree.get sc visited = None.
+Proof.
+  induction scs as [|sc scs]; simpl; intros.
+    congruence.
+
+    inv_mbind_app.
+      apply IHscs in Hfind.
+      destruct Hfind as [scs0 Hfind].
+      destruct_pairs. subst.
+      exists (sc::scs0). 
+      repeat (split; eauto with datatypes v62).
+        intros sc1 Hin. 
+        destruct_in Hin; eauto.
+          congruence.
+        
+      uniq_result.
+      exists nil. repeat (split; eauto with datatypes v62).
+Qed.
+
+Lemma find_next_visit_in_scs_spec: forall visited scs sc scs'
+  (Hfind : Some (sc, scs') = find_next_visit_in_scs visited scs),
+  incl (sc::scs') scs /\ ATree.get sc visited = None.
+Proof.
+  intros.
+  apply find_next_visit_in_scs_spec' in Hfind.
+  destruct_conjs. subst.
+  split; eauto 2 with datatypes v62.
+Qed.
+
+(**********************************************************)
+
+Record PostOrder := mkPO {
+  PO_cnt: positive;
+  PO_a2p: ATree.t positive
+}.
+
+Definition postorder_inc (po:PostOrder) (v:l) : PostOrder :=
+let '(mkPO cnt a2p) := po in
+mkPO (Psucc cnt) (ATree.set v cnt a2p).
+
+Lemma postorder_inc_pres_nonempty: forall po n' n
+  (Hnempty: (PO_a2p po) ! n <> None),
+  (PO_a2p (postorder_inc po n')) ! n <> None.
+Proof.
+  destruct po. simpl.
+  intros.
+  rewrite ATree.gsspec.
+  destruct_if. congruence.
+Qed.
+
+Lemma postorder_inc_eq: forall po n,
+  (PO_a2p (postorder_inc po n)) ! n = Some (PO_cnt po).
+Proof.
+  destruct po; simpl.
+  intros.
+  rewrite ATree.gss; auto.
+Qed.
+
+Lemma postorder_inc_neq: forall po m n (Hneq: m <> n),
+  (PO_a2p (postorder_inc po m)) ! n = (PO_a2p po) ! n.
+Proof.
+  destruct po; simpl.
+  intros.
+  rewrite ATree.gso; auto.
+Qed.
+
+Lemma postorder_inc_lt: forall po a,
+  (PO_cnt po < PO_cnt (postorder_inc po a))%positive.
+Proof.
+  destruct po. simpl. intro. auto with positive.
+Qed.
+
+(*************************************************************)
+
+Fixpoint find_next_visit_in_stk (succs: ATree.t ls)
+  (visited: ATree.t unit) (po:PostOrder) (frs: list Frame) 
+  : l * list Frame * PostOrder + PostOrder :=
+match frs with
+| nil => inr po
+| mkFrame v scs::frs' => 
+    match find_next_visit_in_scs visited scs with
+    | Some (sc, scs') => 
+        inl (sc, mkFrame sc (succs!!!sc)::mkFrame v scs'::frs', po)
+    | None => find_next_visit_in_stk succs visited (postorder_inc po v) frs'
+    end
+end.
+
+Lemma find_next_visit_in_stk_inl_spec: forall succs visited po stk re
+  (Heq: find_next_visit_in_stk succs visited po stk = inl re),
+  stk <> nil.
+Proof.
+  induction stk as [|[v scs] stk]; simpl; intros; congruence.
+Qed.
+
+Lemma find_next_visit_in_scs_none_spec: forall visited sc scs 
+  (Hfind : None = find_next_visit_in_scs visited scs) (Hin: In sc scs),
+  ATree.get sc visited <> None.
+Proof.
+  induction scs as [|sc0 scs]; simpl; intros.
+    congruence.
+
+    destruct Hin as [Hin | Hin]; subst.
+      intro J.
+      rewrite J in Hfind. congruence.
+
+      inv_mbind_app; eauto.
+        congruence.
+Qed.
+
+(**************************************************)
 
 Definition stk_in_children succs (stk : list Frame) : Prop :=
 List.Forall (fun fr : Frame => 
@@ -199,6 +290,26 @@ Proof.
         apply List.in_map with (f:=fst) in H2; auto.
 Qed.
 
+Lemma find_next_visit_in_stk_spec12: forall (succs : ATree.t ls) 
+  (visited : ATree.t unit) (po : PostOrder) (stk : list Frame)
+  (H : stk_in_children succs stk /\
+       incl (XATree.parents_of_tree visited) (XATree.children_of_tree succs))
+  next stk' po'
+  (Heq_anonymous : inl (next, stk', po') =
+                   find_next_visit_in_stk succs visited po stk),
+  stk_in_children succs stk' /\
+  incl (XATree.parents_of_tree (ATree.set next tt visited))
+       (XATree.children_of_tree succs).
+Proof.
+  intros.
+  destruct_conjs.
+  split.
+    eapply find_next_visit_in_stk_spec1; eauto.
+    eapply find_next_visit_in_stk_spec2; eauto.
+Qed.
+
+(************************)
+
 Program Fixpoint dfs_aux1 (succs: ATree.t ls)
   (visited: ATree.t unit) (po:PostOrder) (stk: list Frame) 
   (Hp: stk_in_children succs stk /\
@@ -243,24 +354,6 @@ Definition dfs_aux_F (f: dfs_aux_type)
   end.
 
 Require Import cpdt_tactics.
-
-Lemma find_next_visit_in_stk_spec12: forall (succs : ATree.t ls) 
-  (visited : ATree.t unit) (po : PostOrder) (stk : list Frame)
-  (H : stk_in_children succs stk /\
-       incl (XATree.parents_of_tree visited) (XATree.children_of_tree succs))
-  next stk' po'
-  (Heq_anonymous : inl (next, stk', po') =
-                   find_next_visit_in_stk succs visited po stk),
-  stk_in_children succs stk' /\
-  incl (XATree.parents_of_tree (ATree.set next tt visited))
-       (XATree.children_of_tree succs).
-Proof.
-  intros.
-  destruct_conjs.
-  split.
-    eapply find_next_visit_in_stk_spec1; eauto.
-    eapply find_next_visit_in_stk_spec2; eauto.
-Qed.
 
 Program Fixpoint dfs_aux_terminates (succs: ATree.t ls)
   (visited: ATree.t unit) (po:PostOrder) (stk: list Frame) 
@@ -369,6 +462,173 @@ Proof.
       eauto using le_max_l with arith.
 Qed.
 
+(*************************************************************)
+
+Definition node_in_stk (a2:atom) (stk:list Frame) : Prop :=
+exists stk1, exists stk3, exists scs2, stk = stk1 ++ mkFrame a2 scs2  :: stk3.
+
+Lemma node_in_stk_push: forall a2 hd v scs l1 stk
+  (Hnd: node_in_stk a2 ({| Fr_name := v; Fr_scs := scs |} :: stk)),
+  node_in_stk a2 (hd :: {| Fr_name := v; Fr_scs := l1 |} :: stk).
+Proof.
+  intros.
+  destruct Hnd as [stk1 [stk2 [scs' Hin]]].
+  destruct stk1 as [|fr1 stk1].
+    inv Hin.
+    exists [hd]. exists stk2. exists l1. simpl_env. auto.
+
+    inv Hin.
+    exists (hd::{|Fr_name:=v; Fr_scs:=l1|}::stk1). 
+    exists stk2. exists scs'. simpl_env. auto.
+Qed.
+
+Lemma node_in_stk_hd: forall Fr_name0 Fr_scs0 stk,
+  node_in_stk Fr_name0 ({| Fr_name := Fr_name0; Fr_scs := Fr_scs0 |} :: stk).
+Proof.
+  exists nil. exists stk. exists Fr_scs0. auto.
+Qed.
+
+Lemma node_in_stk_pop: forall a2 v scs fr stk
+  (Hin: node_in_stk a2
+           ({| Fr_name := v; Fr_scs := scs |}
+            :: fr :: stk))
+  (Hneq: a2 <> v),
+  node_in_stk a2 (fr :: stk).
+Proof.
+  intros.
+  destruct Hin as [stk1 [stk2 [scs' Hin]]].
+  destruct stk1 as [|fr1 stk1].
+    inv Hin. congruence.
+
+    inv Hin.
+    rewrite H1. unfold node_in_stk. eauto.
+Qed.
+
+Lemma node_notin_empty_stk: forall a2 (H:node_in_stk a2 nil), False.
+Proof.
+  unfold node_in_stk.
+  intros.
+  destruct_conjs.
+  symmetry in H2.
+  contradict H2.
+  apply app_cons_not_nil.
+Qed.
+
+Lemma node_in_single_stk: forall a2 entry scs
+  (Hnd: node_in_stk a2 ({| Fr_name := entry; Fr_scs := scs |} :: nil)),
+  a2 = entry.
+Proof.
+  unfold node_in_stk.
+  intros.
+  destruct_conjs.
+  destruct Hnd; inv H1; auto.
+    symmetry in H4.
+    contradict H4.
+    apply app_cons_not_nil.
+Qed.
+
+Lemma node_in_stk_cons_inv: forall n hd stk
+  (Hnd: node_in_stk n (hd :: stk)),
+  n = Fr_name hd \/ node_in_stk n stk.
+Proof.
+  unfold node_in_stk.
+  intros.
+  destruct Hnd as [A [B [C Hnd]]].
+  destruct A as [|A]; inv Hnd; eauto.
+Qed.
+
+(*************************************************************)
+
+Module Inv. Section Inv.
+
+Variable wf_stack: ATree.t ls -> ATree.t unit -> PostOrder -> list Frame -> Prop.
+
+Hypothesis find_next_visit_in_stk__wf_stack: forall succs stk visited
+  po (Hwf: wf_stack succs visited po stk) next stk' po'
+  (Heq: find_next_visit_in_stk succs visited po stk = inl (next, stk', po')),
+  wf_stack succs (ATree.set next tt visited) po' stk'.
+
+Variable wf_po: ATree.t ls -> PostOrder -> Prop.
+
+Hypothesis wf_stack__find_next_visit_in_stk_inr__wf_order: forall succs 
+  stk visited po1 (Hwf : wf_stack succs visited po1 stk) po2 
+  (Heq: find_next_visit_in_stk succs visited po1 stk = inr po2),
+  wf_po succs po2.
+
+Definition dfs_aux_wf_prop (n:nat) : Prop := 
+  forall (succs: ATree.t ls) 
+  (visited: ATree.t unit) 
+  (Heq: n = (length (XATree.children_of_tree succs) - 
+             length (XATree.parents_of_tree visited))%nat)
+  (po1:PostOrder) (stk: list Frame) 
+  (Hp: stk_in_children succs stk /\
+       incl (XATree.parents_of_tree visited) (XATree.children_of_tree succs))
+  po2 (Hdfs: dfs_aux succs visited po1 stk Hp = po2)
+  (Hwf: wf_stack succs visited po1 stk),
+  wf_po succs po2.
+
+Lemma dfs_aux_wf_aux: forall n, dfs_aux_wf_prop n.
+Proof.
+  intros.
+  elim n using (well_founded_induction lt_wf).
+  unfold dfs_aux_wf_prop.
+  intros x IH. intros.
+  apply dfs_aux_fix_eqn in Hdfs.
+  caseEq (find_next_visit_in_stk succs visited po1 stk).
+    intros [[next stk'] po'] Hfind; fill_holes_in_ctx.
+    destruct Hdfs as [Hp' Hdfs].
+    eapply IH with (y:=
+      (length (XATree.children_of_tree succs) -
+       length (XATree.parents_of_tree (ATree.set next tt visited)))%nat) 
+      in Hdfs; eauto.
+      subst.  
+      symmetry in Hfind.
+      destruct_conjs.
+      eapply find_next_visit_in_stk_spec3 in Hfind; eauto. 
+
+    intros p Hfind; fill_holes_in_ctx.
+    subst.
+    eapply wf_stack__find_next_visit_in_stk_inr__wf_order; eauto.
+Qed.
+
+Lemma dfs_aux_wf: forall (succs: ATree.t ls) 
+  (visited: ATree.t unit) (po1:PostOrder) (stk: list Frame) 
+  (Hp: stk_in_children succs stk /\
+       incl (XATree.parents_of_tree visited) (XATree.children_of_tree succs))
+  po2 (Hdsf: dfs_aux succs visited po1 stk Hp = po2)
+  (Hwf: wf_stack succs visited po1 stk),
+  wf_po succs po2.
+Proof.
+  intros.
+  assert (J:=@dfs_aux_wf_aux 
+                (length (XATree.children_of_tree succs) - 
+                 length (XATree.parents_of_tree visited))%nat).
+  unfold dfs_aux_wf_prop in J.
+  eauto.
+Qed.
+
+Variable succs: ATree.t ls.
+Variable entry: l.
+Variable pinit: positive.
+
+Hypothesis entry_wf_stack: 
+  wf_stack succs (ATree.empty unit)
+    {| PO_cnt := pinit; PO_a2p := ATree.empty positive |}
+    [{| Fr_name := entry; Fr_scs := succs !!! entry |}].
+
+Lemma dfs_wf: forall po 
+  (Hdfs: dfs succs entry pinit = po), wf_po succs po. 
+Proof.
+  unfold dfs. intros.
+  apply dfs_aux_wf in Hdfs; auto.
+Qed.
+
+End Inv. End Inv.
+
+(*************************************************************)
+
+Module Order.
+
 Fixpoint stk_isa_path (succs: ATree.t ls) (entry:atom) (stk:list Frame) : Prop :=
 match stk with
 | nil => True
@@ -376,9 +636,6 @@ match stk with
 | mkFrame sc _::(mkFrame n _::_) as stk' => 
     In sc (succs !!! n) /\ stk_isa_path succs entry stk'
 end.
-
-Definition node_in_stk (a2:atom) (stk:list Frame) : Prop :=
-exists stk1, exists stk3, exists scs2, stk = stk1 ++ mkFrame a2 scs2  :: stk3.
 
 Definition wf_aorder_aux (succs: ATree.t ls) (entry:atom) (po:PostOrder) 
   (stk: list Frame) : Prop :=
@@ -394,35 +651,17 @@ Definition stk_takes_succs succs (stk : list Frame) : Prop :=
 List.Forall (fun fr : Frame => 
              incl (Fr_scs fr) (succs !!! (Fr_name fr))) stk.
 
-Definition wf_stack (succs: ATree.t ls) (entry:atom) (po:PostOrder) 
+Definition wf_stack (entry:atom) (succs: ATree.t ls) (po:PostOrder) 
   (stk: list Frame) : Prop :=
 stk_isa_path succs entry stk /\
 stk_takes_succs succs stk /\
 wf_aorder_aux succs entry po stk.
 
-Definition wf_aorder scs (entry:atom) (a2p:ATree.t positive) : Prop :=
+Definition wf_aorder (entry:atom) scs (a2p:ATree.t positive) : Prop :=
   forall a1 (Hneq: a1 <> entry) p1 (Hget: a2p ! a1 = Some p1),
   exists a2, exists p2,
     In a2 ((XATree.make_predecessors scs) !!! a1) /\ 
     a2p ! a2 = Some p2 /\ (p2 > p1)%positive.
-
-Definition dfs_aux_wf_stack_prop (n:nat) : Prop := forall (succs: ATree.t ls) 
-  (visited: ATree.t unit) 
-  (Heq: n = (length (XATree.children_of_tree succs) - 
-             length (XATree.parents_of_tree visited))%nat)
-  entry (po1:PostOrder) (stk: list Frame) 
-  (Hp: stk_in_children succs stk /\
-       incl (XATree.parents_of_tree visited) (XATree.children_of_tree succs))
-  po2 (Hdfs: dfs_aux succs visited po1 stk Hp = po2)
-  (Hwf: wf_stack succs entry po1 stk),
-  wf_aorder succs entry (PO_a2p po2).
-
-Lemma find_next_visit_in_stk_inl_spec: forall succs visited po stk re
-  (Heq: find_next_visit_in_stk succs visited po stk = inl re),
-  stk <> nil.
-Proof.
-  induction stk as [|[v scs] stk]; simpl; intros; congruence.
-Qed.
 
 Lemma find_next_visit_in_stk__stk_isa_path: forall succs entry 
   stk (Hwfstk: stk_takes_succs succs stk) visited
@@ -466,21 +705,6 @@ Proof.
           destruct_conjs. apply H. auto with coqlib.
 Qed.
 
-Lemma node_in_stk_push: forall a2 hd v scs l1 stk
-  (Hnd: node_in_stk a2 ({| Fr_name := v; Fr_scs := scs |} :: stk)),
-  node_in_stk a2 (hd :: {| Fr_name := v; Fr_scs := l1 |} :: stk).
-Proof.
-  intros.
-  destruct Hnd as [stk1 [stk2 [scs' Hin]]].
-  destruct stk1 as [|fr1 stk1].
-    inv Hin.
-    exists [hd]. exists stk2. exists l1. simpl_env. auto.
-
-    inv Hin.
-    exists (hd::{|Fr_name:=v; Fr_scs:=l1|}::stk1). 
-    exists stk2. exists scs'. simpl_env. auto.
-Qed.
-
 Lemma push_wf_aorder_aux: forall (entry : atom) (succs : ATree.t ls)
   (v : l) (scs : ls) (stk : list Frame) (next : l) (po' : PostOrder) (l1 : ls)
   (Hwf : wf_aorder_aux succs entry po'
@@ -501,28 +725,6 @@ Proof.
     split; auto.
       destruct J4 as [J4 | J4]; auto.
         right. eapply node_in_stk_push; eauto.
-Qed.
-
-Lemma node_in_stk_hd: forall Fr_name0 Fr_scs0 stk,
-  node_in_stk Fr_name0 ({| Fr_name := Fr_name0; Fr_scs := Fr_scs0 |} :: stk).
-Proof.
-  exists nil. exists stk. exists Fr_scs0. auto.
-Qed.
-
-Lemma node_in_stk_pop: forall a2 v scs fr stk
-  (Hin: node_in_stk a2
-           ({| Fr_name := v; Fr_scs := scs |}
-            :: fr :: stk))
-  (Hneq: a2 <> v),
-  node_in_stk a2 (fr :: stk).
-Proof.
-  intros.
-  destruct Hin as [stk1 [stk2 [scs' Hin]]].
-  destruct stk1 as [|fr1 stk1].
-    inv Hin. congruence.
-
-    inv Hin.
-    rewrite H1. unfold node_in_stk. eauto.
 Qed.
 
 Lemma pop_wf_aorder_aux: forall (entry : atom) (succs : ATree.t ls)
@@ -602,9 +804,9 @@ Proof.
 Qed.
 
 Lemma find_next_visit_in_stk__wf_stack: forall entry succs stk visited
-  po (Hwf: wf_stack succs entry po stk) next stk' po'
+  po (Hwf: wf_stack entry succs po stk) next stk' po'
   (Heq: find_next_visit_in_stk succs visited po stk = inl (next, stk', po')),
-  wf_stack succs entry po' stk'.
+  wf_stack entry succs po' stk'.
 Proof.
   intros.
   destruct Hwf as [J1 [J2 J3]]. 
@@ -614,34 +816,11 @@ Proof.
   eapply find_next_visit_in_stk__stk_takes_succs in J2; eauto.
 Qed.
 
-Lemma node_notin_empty_stk: forall a2 (H:node_in_stk a2 nil), False.
-Proof.
-  unfold node_in_stk.
-  intros.
-  destruct_conjs.
-  symmetry in H2.
-  contradict H2.
-  apply app_cons_not_nil.
-Qed.
-
-Lemma node_in_single_stk: forall a2 entry scs
-  (Hnd: node_in_stk a2 ({| Fr_name := entry; Fr_scs := scs |} :: nil)),
-  a2 = entry.
-Proof.
-  unfold node_in_stk.
-  intros.
-  destruct_conjs.
-  destruct Hnd; inv H1; auto.
-    symmetry in H4.
-    contradict H4.
-    apply app_cons_not_nil.
-Qed.
-
 Lemma wf_aorder_aux__find_next_visit_in_stk_inr__wf_aorder: forall 
   succs entry stk po1 (Hwf': stk_isa_path succs entry stk)
   (Hwf : wf_aorder_aux succs entry po1 stk) po2 visited
   (Heq: find_next_visit_in_stk succs visited po1 stk = inr po2),
-  wf_aorder succs entry (PO_a2p po2).
+  wf_aorder entry succs (PO_a2p po2).
 Proof.
   induction stk as [|[v scs] stk]; simpl; intros.
     uniq_result.
@@ -686,69 +865,37 @@ Proof.
 Qed.
 
 Lemma wf_stack__find_next_visit_in_stk_inr__wf_aorder: forall succs entry po1 stk
-  (Hwf : wf_stack succs entry po1 stk) po2 visited
+  (Hwf : wf_stack entry succs po1 stk) po2 visited
   (Heq: find_next_visit_in_stk succs visited po1 stk = inr po2),
-  wf_aorder succs entry (PO_a2p po2).
+  wf_aorder entry succs (PO_a2p po2).
 Proof.
   intros.
   destruct Hwf as [J1 [J2 J3]].
   eapply wf_aorder_aux__find_next_visit_in_stk_inr__wf_aorder; eauto.
 Qed.
 
-Lemma dfs_aux_wf_stack_aux: forall n, dfs_aux_wf_stack_prop n.
+Lemma entry_wf_stack: forall scs entry pinit,
+  wf_stack entry scs {| PO_cnt := pinit; PO_a2p := ATree.empty positive |}
+     [{| Fr_name := entry; Fr_scs := scs !!! entry |}].
 Proof.
   intros.
-  elim n using (well_founded_induction lt_wf).
-  unfold dfs_aux_wf_stack_prop.
-  intros x IH. intros.
-  apply dfs_aux_fix_eqn in Hdfs.
-  caseEq (find_next_visit_in_stk succs visited po1 stk).
-    intros [[next stk'] po'] Hfind; fill_holes_in_ctx.
-    destruct Hdfs as [Hp' Hdfs].
-    eapply IH with (y:=
-      (length (XATree.children_of_tree succs) -
-       length (XATree.parents_of_tree (ATree.set next tt visited)))%nat) 
-      in Hdfs; eauto.
-      subst.  
-      symmetry in Hfind.
-      destruct_conjs.
-      eapply find_next_visit_in_stk_spec3 in Hfind; eauto. 
-
-      eapply find_next_visit_in_stk__wf_stack; eauto. 
-
-    intros p Hfind; fill_holes_in_ctx.
-    subst.
-    eapply wf_stack__find_next_visit_in_stk_inr__wf_aorder; eauto.
-Qed.
-
-Lemma dfs_aux_wf_stack: forall (succs: ATree.t ls) entry
-  (visited: ATree.t unit) (po1:PostOrder) (stk: list Frame) 
-  (Hp: stk_in_children succs stk /\
-       incl (XATree.parents_of_tree visited) (XATree.children_of_tree succs))
-  po2 (Hdsf: dfs_aux succs visited po1 stk Hp = po2)
-  (Hwf: wf_stack succs entry po1 stk),
-  wf_aorder succs entry (PO_a2p po2).
-Proof.
-  intros.
-  assert (J:=@dfs_aux_wf_stack_aux 
-                (length (XATree.children_of_tree succs) - 
-                 length (XATree.parents_of_tree visited))%nat).
-  unfold dfs_aux_wf_stack_prop in J.
-  eauto.
-Qed.
-
-Lemma dfs_wf_order: forall scs entry pinit po (Hdfs: dfs scs entry pinit = po),
-  wf_aorder scs entry (PO_a2p po).
-Proof.
-  unfold dfs. intros.
-  apply dfs_aux_wf_stack with (entry:=entry) in Hdfs; auto.
   split. constructor; auto.
   split. 
     constructor; simpl; auto.
       intro x. auto.
-
     intros a1 p1 Hget.   
     rewrite ATree.gempty in Hget. congruence.
+Qed.
+
+Lemma dfs_wf_order: forall scs entry pinit po (Hdfs: dfs scs entry pinit = po),
+  wf_aorder entry scs (PO_a2p po).
+Proof.
+  intros.
+  eapply Inv.dfs_wf with 
+    (wf_stack:=fun succs visited po stk => wf_stack entry succs po stk)
+    (wf_po:=fun succs po => wf_aorder entry succs (PO_a2p po)); 
+    eauto using wf_stack__find_next_visit_in_stk_inr__wf_aorder,
+                find_next_visit_in_stk__wf_stack, entry_wf_stack.
 Qed.
 
 Definition wf_porder scs (entry:positive): Prop :=
@@ -757,11 +904,13 @@ Definition wf_porder scs (entry:positive): Prop :=
    (p > n)%positive.
 
 Lemma asuccs_psuccs_pres_order: forall ascs pscs aentry pentry a2p
-  (Htrans: asuccs_psuccs a2p ascs = pscs) (Hwf: wf_aorder ascs aentry a2p)
+  (Htrans: asuccs_psuccs a2p ascs = pscs) (Hwf: wf_aorder aentry ascs a2p)
   (Hentry: a2p ! aentry = Some pentry),
   wf_porder pscs pentry.
-Admitted.
+Admitted. (* asuccs_psuccs *)
  
+End Order.
+
 (************************)
 
 Require Import Dipaths.
@@ -770,21 +919,780 @@ Section VertexArc.
 
 Variable successors: ATree.t (list atom).
 
-Definition vertexes' : V_set :=
+Definition vertexes : V_set :=
 fun (v:Vertex) => let '(index n) := v in XATree.in_cfg successors n.
 
-Definition arcs' : A_set :=
+Definition arcs : A_set :=
 fun (arc:Arc) =>
   let '(A_ends (index n2) (index n1)) := arc in
   In n2 (successors!!!n1).
 
-Definition reachable' entry av : Prop :=
-  exists vl: V_list, exists al: A_list, D_walk vertexes' arcs' av entry vl al.
+Definition reachable entry av : Prop :=
+  exists vl: V_list, exists al: A_list, D_walk vertexes arcs av entry vl al.
+
+Lemma reachable_succ: forall (entry : ATree.elt) 
+  (fr : l) (next : l) (H1 : reachable (index entry) (index fr))
+  (Hscs : In next successors !!! fr),
+  reachable (index entry) (index next).
+Proof.
+  intros.
+  destruct H1 as [vl [al Hwk]].
+  exists (index fr::vl). exists (A_ends (index next) (index fr)::al).
+  apply DW_step; auto.
+    apply XATree.in_succ__in_cfg with (p:=fr); auto.
+Qed.
+
+Lemma reachable_entry: forall (entry : ATree.elt) 
+  (Hincfg: XATree.in_cfg successors entry),
+  reachable (index entry) (index entry).
+Proof.
+  intros.
+  exists V_nil. exists A_nil. 
+  constructor; auto.
+Qed.
 
 End VertexArc.
 
-Lemma dfs_reachable: forall scs entry pinit po (Hdfs: dfs scs entry pinit = po),
+(************************)
+
+Module ReachableEntry. 
+
+Definition wf_stack entry (po:PostOrder) (stk: list Frame) : Prop :=
+  (exists others, exists esuccs, 
+     stk = others ++ [mkFrame entry esuccs]) \/
+  (PO_a2p po) ! entry <> None.
+
+Definition wf_order entry (po:PostOrder) : Prop :=
+  (PO_a2p po) ! entry <> None.
+
+Lemma pop__wf_stack: forall (entry : l) (fr : l) (todo : ls)
+  (stk : list Frame) (po1 : PostOrder)
+  (Hwf : wf_stack entry po1 ({| Fr_name := fr; Fr_scs := todo |} :: stk)),
+  wf_stack entry (postorder_inc po1 fr) stk.
+Proof.
+  unfold wf_stack.
+  intros.
+  destruct Hwf as [Hwf | Hwf].
+  SCase "1".
+    destruct Hwf as [others [esuccs Hwf]].
+    destruct others as [|F others]; inv Hwf; eauto.
+      rewrite postorder_inc_eq. right. congruence. 
+  SCase "2".
+    right. apply postorder_inc_pres_nonempty; auto.
+Qed.
+
+Lemma find_next_visit_in_stk__wf_stack: forall succs entry stk visited
+  po (Hwf: wf_stack entry po stk) next stk' po'
+  (Heq: find_next_visit_in_stk succs visited po stk = inl (next, stk', po')),
+  wf_stack entry po' stk'.
+Proof.
+  unfold wf_stack.
+  induction stk as [|[fr todo] stk]; simpl; intros.
+    congruence.
+
+    inv_mbind_app.
+    Case "push".
+      destruct_let. uniq_result.
+      destruct Hwf as [Hwf | Hwf]; auto.
+        left. 
+        destruct Hwf as [others [esuccs Hwf]].
+        destruct others as [|F others]; inv Hwf. 
+          simpl_env. eauto.
+          exists ({| Fr_name := next; Fr_scs := succs !!! next |}::
+                  {| Fr_name := fr; Fr_scs := l1 |}::others).
+          exists esuccs. simpl_env. auto.     
+
+    Case "pop".
+      apply IHstk in Heq; auto.
+        eapply pop__wf_stack; eauto.
+Qed.
+
+Lemma wf_stack__find_next_visit_in_stk_inr__wf_aorder: forall succs entry stk po1
+  (Hwf : wf_stack entry po1 stk) po2 visited
+  (Heq: find_next_visit_in_stk succs visited po1 stk = inr po2),
+  wf_order entry po2.
+Proof.
+  induction stk as [|[fr todo] stk]; simpl; intros.
+    uniq_result. 
+    destruct Hwf as [|]; auto.
+    destruct_conjs. uniq_result'. inv H2.
+    
+    inv_mbind_app.
+      destruct_let. congruence.
+      apply IHstk in Heq; auto.
+        eapply pop__wf_stack; eauto.
+Qed.
+
+Lemma entry_wf_stack: forall scs entry pinit,
+  wf_stack entry {| PO_cnt := pinit; PO_a2p := ATree.empty positive |}
+     [{| Fr_name := entry; Fr_scs := scs !!! entry |}].
+Proof.
+  intros.
+  left. exists nil. exists scs!!!entry. auto.
+Qed.
+
+Lemma dfs_wf: forall scs entry pinit po 
+  (Hdfs: dfs scs entry pinit = po), (PO_a2p po) ! entry <> None.
+Proof.
+  intros.
+  eapply Inv.dfs_wf with 
+    (wf_stack:=fun succs visited po stk => wf_stack entry po stk)
+    (wf_po:=fun succs po => wf_order entry po); 
+    eauto using wf_stack__find_next_visit_in_stk_inr__wf_aorder,
+                find_next_visit_in_stk__wf_stack, entry_wf_stack.
+Qed.
+ 
+End ReachableEntry. 
+
+(************************)
+
+Require Import Program.Equality.
+
+Module ReachableSucc. 
+
+Definition succ_of_numbered_is_visited_or_numbered (succs: ATree.t ls)
+  (visited: ATree.t unit) (po:PostOrder): Prop :=
+  forall n sc (Hnn: (PO_a2p po) ! n <> None) (Hinsc: In sc (succs !!! n)),
+    visited ! sc <> None \/ (PO_a2p po) ! sc <> None.
+
+Definition visited_is_numbered_or_stked (visited: ATree.t unit) (po:PostOrder) 
+  (stk: list Frame) : Prop :=
+  forall n (Hvisited: visited ! n <> None),
+    (PO_a2p po) ! n <> None \/ node_in_stk n stk.
+
+Definition wf_succs_of_fr succs (visited: ATree.t unit) (po:PostOrder) 
+  (fr : Frame) : Prop :=
+forall sc (Hin: In sc (succs !!! (Fr_name fr))),
+  visited ! sc <> None \/ (PO_a2p po) ! sc <> None \/ In sc (Fr_scs fr).
+
+Definition wf_succs_of_stk succs (visited: ATree.t unit) (po:PostOrder) 
+  (stk : list Frame): Prop :=
+List.Forall (wf_succs_of_fr succs visited po) stk.
+
+Definition wf_stack (succs: ATree.t ls) (visited: ATree.t unit) (po:PostOrder) 
+  (stk: list Frame) : Prop :=
+  succ_of_numbered_is_visited_or_numbered succs visited po /\
+  visited_is_numbered_or_stked visited po stk /\
+  wf_succs_of_stk succs visited po stk.
+
+Lemma pushed__wf_succs_of_fr: forall succs visited po next,
+  wf_succs_of_fr succs visited po 
+    {| Fr_name := next; Fr_scs := succs !!! next |}.
+Proof.
+  intros. intros n Hin. simpl. auto.
+Qed.
+
+Hint Unfold wf_succs_of_fr.
+
+Lemma wf_succs_of_stk__postorder_inc: forall n succs visited po stk
+  (Hwf: wf_succs_of_stk succs visited po stk),
+  wf_succs_of_stk succs visited (postorder_inc po n) stk.
+Proof.
+  unfold wf_succs_of_stk.
+  intros.
+  dependent induction Hwf; auto.
+    constructor; auto.
+      autounfold. intros.
+      apply H in Hin.
+      destruct Hin as [Hin | [Hin | Hin]]; auto.
+        right. left.
+        eapply postorder_inc_pres_nonempty in Hin; eauto.
+Qed.
+
+Lemma wf_succs_of_stk__visited_inc: forall next succs visited po stk
+  (Hwf: wf_succs_of_stk succs visited po stk),
+  wf_succs_of_stk succs (ATree.set next tt visited) po stk.
+Proof.
+  unfold wf_succs_of_stk.
+  intros.
+  dependent induction Hwf; auto.
+    constructor; auto.
+      autounfold. intros.
+      apply H in Hin.
+      destruct Hin as [Hin | [Hin | Hin]]; auto.
+        left. apply ATree_set_pres_nonempty; auto.
+Qed.
+
+Lemma find_next_visit_in_stk__wf_succs_of_stk: forall succs stk visited po
+  (Hwf: wf_succs_of_stk succs visited po stk) next stk' po'
+  (Heq: find_next_visit_in_stk succs visited po stk = inl (next, stk', po')),
+  wf_succs_of_stk succs (ATree.set next tt visited) po' stk'.
+Proof.
+  induction stk as [|[fr todo] stk]; simpl; intros.
+  Case "base".
+    congruence.
+
+  Case "ind".
+    inv_mbind_app.
+    SCase "push".
+      destruct_let. uniq_result.
+      inv Hwf.
+      constructor.
+      SSCase "new fr".
+        apply pushed__wf_succs_of_fr.
+      constructor.
+      SSCase "old hd".
+        apply find_next_visit_in_scs_spec' in HeqR.
+        destruct HeqR as [scs0 [J1 [J2 J3]]]; subst.
+        intros n Hin. 
+        apply H1 in Hin.
+        destruct Hin as [Hin | [Hin | Hin]]; auto.
+        SSSCase "1".
+          left. apply ATree_set_pres_nonempty; auto.
+        SSSCase "2".
+          simpl in Hin. simpl.
+          destruct_in Hin.
+            left. apply ATree_set_pres_nonempty; auto.
+          destruct_in Hin.
+            left. rewrite ATree.gss. congruence.
+      SSCase "old tl".
+        apply wf_succs_of_stk__visited_inc; auto.
+
+    SCase "pop".
+      apply IHstk in Heq; auto.
+        inv Hwf.
+        apply wf_succs_of_stk__postorder_inc; auto.
+Qed.
+
+Lemma find_next_visit_in_scs_none__succ_of_numbered_is_visited_or_numbered: 
+  forall (succs : ATree.t ls) (visited : ATree.t unit) (po : PostOrder)
+  (fr : l) (todo : ls) (stk : list Frame) 
+  (J1 : succ_of_numbered_is_visited_or_numbered succs visited po)
+  (J3 : wf_succs_of_fr succs visited po {| Fr_name := fr; Fr_scs := todo |})
+  (Hnone : None = find_next_visit_in_scs visited todo),
+  succ_of_numbered_is_visited_or_numbered succs visited
+     (postorder_inc po fr).
+Proof.
+  intros.
+  intros n sc Hnn Hinsc.
+  destruct po. simpl in *.
+  destruct (eq_atom_dec fr n); subst.
+  SCase "fr = n".
+    apply J3 in Hinsc.
+    destruct Hinsc as [Hinsc | Hinsc]; auto.
+    destruct Hinsc as [Hinsc | Hinsc].
+    SSCase "1.1.1".
+      rewrite ATree.gss in Hnn.
+      right.
+      rewrite ATree.gsspec.
+      destruct_if.
+  
+    SSCase "1.1.2".
+      eapply find_next_visit_in_scs_none_spec in Hnone; eauto.
+  
+  SCase "fr <> n".
+    rewrite ATree.gso in Hnn; auto.
+    apply J1 in Hinsc; auto.
+    destruct Hinsc as [Hinsc | Hinsc]; auto.
+    simpl in Hinsc.
+    right.
+    rewrite ATree.gsspec.
+    destruct_if. congruence.
+Qed.
+
+Lemma find_next_visit_in_stk__succ_of_numbered_is_visited_or_numbered: 
+  forall succs stk visited po
+  (Hwf': wf_succs_of_stk succs visited po stk)
+  (Hwf: succ_of_numbered_is_visited_or_numbered succs visited po) next stk' po'
+  (Heq: find_next_visit_in_stk succs visited po stk = inl (next, stk', po')),
+  succ_of_numbered_is_visited_or_numbered succs (ATree.set next tt visited) po'.
+Proof.
+  induction stk as [|[fr todo] stk]; simpl; intros.
+  Case "base".
+    congruence.
+
+  Case "ind".
+    inv_mbind_app.
+    SCase "push".
+      destruct_let. uniq_result.
+      intros n sc Hnn Hinsc.
+      apply Hwf in Hinsc; auto.
+      destruct Hinsc as [Hinsc | Hinsc]; auto.
+        left. apply ATree_set_pres_nonempty; auto.
+
+    SCase "pop".
+      inv Hwf'.
+      apply IHstk in Heq; auto.
+        apply wf_succs_of_stk__postorder_inc; auto.
+        eapply find_next_visit_in_scs_none__succ_of_numbered_is_visited_or_numbered;
+          eauto.
+Qed.
+
+Lemma visited_is_numbered_or_stked__postorder_inc: forall 
+  (visited : ATree.t unit) (po : PostOrder) (fr : l) (todo : ls)
+  (stk : list Frame)
+  (J2 : visited_is_numbered_or_stked visited po
+         ({| Fr_name := fr; Fr_scs := todo |} :: stk)),
+  visited_is_numbered_or_stked visited (postorder_inc po fr) stk.
+Proof.
+  intros.
+  intros n Hnv.
+  apply J2 in Hnv.
+  destruct Hnv as [Hnv | Hnv].
+  SCase "2.1".
+    left. apply postorder_inc_pres_nonempty; auto.
+  SCase "2.2".
+    apply node_in_stk_cons_inv in Hnv.
+    destruct Hnv as [Hinv | Hinv]; subst; auto.
+      simpl. left.
+      rewrite postorder_inc_eq. congruence.        
+Qed.
+
+Lemma find_next_visit_in_stk__visited_is_numbered_or_stked: 
+  forall succs stk visited po
+  (Hwf: visited_is_numbered_or_stked visited po stk) next stk' po'
+  (Heq: find_next_visit_in_stk succs visited po stk = inl (next, stk', po')),
+  visited_is_numbered_or_stked (ATree.set next tt visited) po' stk'.
+Proof.
+  induction stk as [|[fr todo] stk]; simpl; intros.
+  Case "base".
+    congruence.
+
+  Case "ind".
+    inv_mbind_app.
+    SCase "push".
+      destruct_let. uniq_result.
+      intros n Hinv.
+      rewrite ATree.gsspec in Hinv.
+      destruct_if; subst.
+      SSCase "1".
+        right. apply node_in_stk_hd.
+      SSCase "2".
+        apply Hwf in Hinv.
+        destruct Hinv as [Hinv | Hinv]; auto.
+        eapply node_in_stk_push in Hinv; eauto.
+
+    SCase "pop".
+      apply IHstk in Heq; auto.
+        eapply visited_is_numbered_or_stked__postorder_inc; eauto.
+Qed.
+
+Lemma find_next_visit_in_stk__wf_stack: forall succs stk visited
+  po (Hwf: wf_stack succs visited po stk) next stk' po'
+  (Heq: find_next_visit_in_stk succs visited po stk = inl (next, stk', po')),
+  wf_stack succs (ATree.set next tt visited) po' stk'.
+Proof.
+  intros.
+  destruct Hwf as [J1 [J2 J3]]. 
+  unfold wf_stack.
+  eapply find_next_visit_in_stk__succ_of_numbered_is_visited_or_numbered 
+    in J1; eauto.
+  eapply find_next_visit_in_stk__visited_is_numbered_or_stked in J2; eauto.
+  eapply find_next_visit_in_stk__wf_succs_of_stk in J3; eauto.
+Qed.
+
+Lemma find_next_visit_in_scs_none__wf_stack: forall succs visited po fr todo stk
+  (Hwf : wf_stack succs visited po ({| Fr_name := fr; Fr_scs := todo |} :: stk))
+  (po2 : PostOrder)
+  (Hnone : None = find_next_visit_in_scs visited todo),
+  wf_stack succs visited (postorder_inc po fr) stk.
+Proof.
+  intros. 
+  destruct Hwf as [J1 [J2 J3]]. 
+  split.
+    inv J3.
+    eapply find_next_visit_in_scs_none__succ_of_numbered_is_visited_or_numbered;
+      eauto.
+  split.
+    eapply visited_is_numbered_or_stked__postorder_inc; eauto.
+    inv J3. apply wf_succs_of_stk__postorder_inc; auto.    
+Qed.
+
+Definition wf_order (succs: ATree.t ls) (po:PostOrder) : Prop :=
+  forall n sc (Hnn: (PO_a2p po) ! n <> None) (Hinsc: In sc (succs !!! n)),
+    (PO_a2p po) ! sc <> None.
+
+Lemma wf_stack__find_next_visit_in_stk_inr__wf_order: forall succs 
+  stk visited po1 (Hwf : wf_stack succs visited po1 stk) po2 
+  (Heq: find_next_visit_in_stk succs visited po1 stk = inr po2),
+  wf_order succs po2.
+Proof.
+  induction stk as [|[fr todo] stk]; simpl; intros.
+  Case "base".
+    uniq_result.
+    destruct Hwf as [J1 [J2 J3]].
+    intros n sc Hnn Hinsc.
+    apply J1 in Hinsc; auto.
+    destruct Hinsc as [Hinsc | Hinsc]; auto.
+    apply J2 in Hinsc.
+    destruct Hinsc as [Hinsc | Hinsc]; auto.
+    apply node_notin_empty_stk in Hinsc. tauto.
+
+  Case "ind".
+    inv_mbind_app.
+      destruct_let. congruence.
+     
+      eapply IHstk; eauto using find_next_visit_in_scs_none__wf_stack.
+Qed.
+
+Lemma entry_wf_stack: forall scs entry pinit,
+  wf_stack scs (ATree.empty unit)
+    {| PO_cnt := pinit; PO_a2p := ATree.empty positive |}
+    [{| Fr_name := entry; Fr_scs := scs !!! entry |}].
+Proof.
+  intros.
+  split. 
+    intros n' sc' Hnn' Hinsc'. 
+    simpl in Hnn'.
+    rewrite ATree.gempty in Hnn'. congruence.
+  split. 
+    intros n' Hv'.
+    rewrite ATree.gempty in Hv'. congruence.
+      
+           constructor; auto.
+Qed.
+
+Lemma dfs_wf: forall scs entry pinit po 
+  (Hdfs: dfs scs entry pinit = po) n sc (Hnn: (PO_a2p po) ! n <> None)
+  (Hinsc: In sc scs!!!n), (PO_a2p po) ! sc <> None.
+Proof.
+  intros until 1.
+  eapply Inv.dfs_wf with (wf_stack:=wf_stack)(wf_po:=wf_order) in Hdfs; 
+    eauto using wf_stack__find_next_visit_in_stk_inr__wf_order,
+                find_next_visit_in_stk__wf_stack, entry_wf_stack.
+Qed.
+
+End ReachableSucc. 
+
+(************************)
+
+Module NumberedAreReachable. 
+
+Definition frame_is_reachable entry (succs: ATree.t ls) (fr: Frame) := 
+  reachable succs (index entry) (index (Fr_name fr)).
+
+Hint Unfold frame_is_reachable. 
+
+Definition frames_are_reachable entry (succs: ATree.t ls) (stk: list Frame) := 
+  List.Forall (frame_is_reachable entry succs) stk.
+
+Definition wf_order entry succs po : Prop :=
+  forall n (Hnn: (PO_a2p po) ! n <> None), 
+    reachable succs (index entry) (index n).
+
+Definition wf_stack entry (succs: ATree.t ls) (po:PostOrder) 
+  (stk: list Frame) : Prop :=
+  Order.stk_takes_succs succs stk /\
+  frames_are_reachable entry succs stk /\
+  wf_order entry succs po.
+
+Lemma find_next_visit_in_stk__frames_are_reachable: 
+  forall entry succs stk visited po
+  (Hpath: Order.stk_takes_succs succs stk)
+  (Hwf: frames_are_reachable entry succs stk) next stk' po'
+  (Heq: find_next_visit_in_stk succs visited po stk = inl (next, stk', po')),
+  frames_are_reachable entry succs stk'.
+Proof.
+  induction stk as [|[fr todo] stk]; simpl; intros.
+    congruence.
+
+    inv Hwf. inv Hpath. simpl in *.
+    inv_mbind_app; eauto.
+      destruct_let. uniq_result.
+        constructor.
+          assert (In next succs !!! fr) as Hscs.
+            apply find_next_visit_in_scs_spec in HeqR.
+            destruct_conjs. auto with coqlib.
+          simpl.
+          eapply reachable_succ; eauto.
+        constructor; auto.
+Qed.
+
+Lemma wf_order__postorder_inc: forall entry succs po fr
+  (Hreach: frame_is_reachable entry succs fr)
+  (Hwf : wf_order entry succs po),
+  wf_order entry succs (postorder_inc po (Fr_name fr)).
+Proof.
+  intros. intros n Hnn.
+  destruct po. simpl in *.
+  rewrite ATree.gsspec in Hnn.
+  destruct_if; subst; auto.
+Qed.
+
+Lemma find_next_visit_in_stk__wf_order: 
+  forall entry succs stk visited po
+  (Hwf': frames_are_reachable entry succs stk)
+  (Hwf: wf_order entry succs po) next stk' po'
+  (Heq: find_next_visit_in_stk succs visited po stk = inl (next, stk', po')),
+  wf_order entry succs po'.
+Proof.
+  induction stk as [|[fr todo] stk]; simpl; intros.
+    congruence.
+
+    inv_mbind_app.
+    Case "push".
+      destruct_let. uniq_result. auto.
+    Case "pop".
+      inv Hwf'.
+      eapply wf_order__postorder_inc in H1; eauto.
+Qed.
+
+Lemma find_next_visit_in_stk__wf_stack: forall entry succs stk visited
+  po (Hwf: wf_stack entry succs po stk) next stk' po'
+  (Heq: find_next_visit_in_stk succs visited po stk = inl (next, stk', po')),
+  wf_stack entry succs po' stk'.
+Proof.
+  intros.
+  destruct Hwf as [J0 [J1 J2]]. 
+  unfold wf_stack.
+  eapply find_next_visit_in_stk__wf_order in J2; eauto.
+  eapply find_next_visit_in_stk__frames_are_reachable in J1; eauto.
+  eapply Order.find_next_visit_in_stk__stk_takes_succs in J0; eauto.
+Qed.
+
+Lemma wf_stack__find_next_visit_in_stk_inr__wf_order: forall entry succs 
+  stk visited po1 (Hwf : wf_stack entry succs po1 stk) po2 
+  (Heq: find_next_visit_in_stk succs visited po1 stk = inr po2),
+  wf_order entry succs po2.
+Proof.
+  unfold wf_stack.
+  induction stk as [|[fr todo] stk]; simpl; intros.
+    uniq_result. tauto.
+
+    inv_mbind_app.
+      destruct_let. congruence.
+
+      apply IHstk in Heq; auto.      
+        destruct Hwf as [Hwf1 [Hwf2 Hwf3]].
+        inv Hwf1. inv Hwf2.
+        split; auto.
+        split; auto.
+          eapply wf_order__postorder_inc in H3; eauto.
+Qed.
+
+Lemma entry_wf_stack: forall scs entry pinit
+  (Hincfg: XATree.in_cfg scs entry),
+  wf_stack entry scs
+    {| PO_cnt := pinit; PO_a2p := ATree.empty positive |}
+    [{| Fr_name := entry; Fr_scs := scs !!! entry |}].
+Proof.
+  intros.
+  split. 
+    constructor; auto.
+      intro x. auto.
+  split.
+    constructor; auto.
+      apply reachable_entry; auto.
+    intros n Hnn. simpl in Hnn.
+    rewrite ATree.gempty in Hnn. congruence.
+Qed.
+
+Lemma dfs_wf: forall scs entry pinit po 
+  (Hincfg: XATree.in_cfg scs entry)
+  (Hdfs: dfs scs entry pinit = po) n (Hnn: (PO_a2p po) ! n <> None),
+  reachable scs (index entry) (index n).
+Proof.
+  intros until 2.
+  eapply Inv.dfs_wf with 
+    (wf_stack:=fun scs v po stk=>wf_stack entry scs po stk)
+    (wf_po:=wf_order entry) in Hdfs; 
+    eauto using wf_stack__find_next_visit_in_stk_inr__wf_order,
+                find_next_visit_in_stk__wf_stack, entry_wf_stack.
+Qed.
+
+End NumberedAreReachable. 
+
+(************************)
+
+Lemma dfs_reachable_complete: forall scs entry pinit po 
+  (Hdfs: dfs scs entry pinit = po) l0
+  (Hreach: reachable scs (index entry) (index l0)),
+  (PO_a2p po) ! l0 <> None.
+Proof.
+  unfold reachable.
+  intros.
+  destruct Hreach as [vl [al Hreach]].
+  dependent induction Hreach.
+    eapply ReachableEntry.dfs_wf; eauto.
+
+    destruct y as [y].
+    eapply ReachableSucc.dfs_wf with (n:=y); eauto.
+Qed.
+
+Lemma dfs_reachable_sound: forall scs entry pinit po 
+  (Hincfg: XATree.in_cfg scs entry)
+  (Hdfs: dfs scs entry pinit = po) l0
+  (Hnn: (PO_a2p po) ! l0 <> None),
+  reachable scs (index entry) (index l0).
+Proof.
+  intros.
+  eapply NumberedAreReachable.dfs_wf; eauto.
+Qed.
+
+Lemma dfs_unreachable_iff_get_none: forall scs entry pinit po 
+  (Hdfs: dfs scs entry pinit = po) (Hincfg: XATree.in_cfg scs entry),
   forall l0, 
-  ~ reachable' scs (index entry) (index l0) <-> (PO_a2p po) ! l0 = None.
-Admitted.
+  ~ reachable scs (index entry) (index l0) <-> (PO_a2p po) ! l0 = None.
+Proof.
+  intros.
+  split; intro J.
+    remember (PO_a2p po) ! l0 as R.
+    destruct R; auto.
+    contradict J.
+    eapply dfs_reachable_sound; try solve [eauto | congruence].
+
+    intro G.
+    eapply dfs_reachable_complete in G; eauto.
+Qed.
+
+Lemma dfs_reachable_iff_get_some: forall scs entry pinit po 
+  (Hdfs: dfs scs entry pinit = po) (Hincfg: XATree.in_cfg scs entry),
+  forall l0, 
+  reachable scs (index entry) (index l0) <-> exists p, (PO_a2p po) ! l0 = Some p.
+Proof.
+  intros.
+  split; intro J.
+    eapply dfs_reachable_complete in J; eauto.
+    destruct (PO_a2p po)!l0; eauto. congruence.
+
+    destruct_conjs.
+    eapply dfs_reachable_sound; try solve [eauto | congruence].
+Qed.
+
+(************************)
+
+Module Injective. 
+
+Definition a2p_injective po : Prop :=
+  forall (p:positive) a1 a2
+  (Hget2 : (PO_a2p po) ! a2 = Some p) (Hget1 : (PO_a2p po) ! a1 = Some p),
+  a1 = a2.
+
+Definition a2p_lt_cnt po : Prop :=
+  forall p a (Hget: (PO_a2p po) ! a = Some p), (p < PO_cnt po)%positive.
+
+Definition wf_order po : Prop :=
+  a2p_lt_cnt po /\ a2p_injective po. 
+
+Lemma a2p_injective__postorder_inc: forall po fr (Hlt: a2p_lt_cnt po)
+  (Hinj: a2p_injective po),
+  a2p_injective (postorder_inc po fr).
+Proof.
+  intros.
+  intros p a1 a2 Hget2 Hget1.
+  destruct (eq_atom_dec fr a2); subst.
+    rewrite postorder_inc_eq in Hget2. uniq_result.
+    destruct (eq_atom_dec a2 a1); subst; auto.
+    rewrite postorder_inc_neq in Hget1; auto.
+    apply Hlt in Hget1. contradict Hget1. apply Plt_irrefl.
+
+    rewrite postorder_inc_neq in Hget2; auto.
+    destruct (eq_atom_dec fr a1); subst.
+      rewrite postorder_inc_eq in Hget1. uniq_result.
+      apply Hlt in Hget2. contradict Hget2. apply Plt_irrefl.
+ 
+      rewrite postorder_inc_neq in Hget1; auto.
+      eapply Hinj; eauto.
+Qed.
+
+Lemma a2p_lt_cnt__postorder_inc: forall po fr (Hlt: a2p_lt_cnt po),
+  a2p_lt_cnt (postorder_inc po fr).
+Proof.
+  intros.
+  intros p a Hget.
+  destruct (eq_atom_dec fr a); subst.
+    rewrite postorder_inc_eq in Hget. uniq_result.
+    apply postorder_inc_lt.
+
+    rewrite postorder_inc_neq in Hget; auto.
+    apply Hlt in Hget.
+    assert (J:=postorder_inc_lt po fr).
+    eapply Plt_trans; eauto.
+Qed.
+
+Lemma find_next_visit_in_stk__a2p_injective: 
+  forall succs stk visited po (Hwf: a2p_injective po) (Hlt: a2p_lt_cnt po) 
+  next stk' po'
+  (Heq: find_next_visit_in_stk succs visited po stk = inl (next, stk', po')),
+  a2p_injective po'.
+Proof.
+  induction stk as [|[fr todo] stk]; simpl; intros.
+    congruence.
+
+    inv_mbind_app.
+    Case "push".
+      destruct_let. uniq_result. auto.
+    Case "pop".
+      apply IHstk in Heq; auto using a2p_injective__postorder_inc,
+                                     a2p_lt_cnt__postorder_inc.
+Qed.
+
+Lemma find_next_visit_in_stk__a2p_lt_cnt: 
+  forall succs stk visited po (Hlt: a2p_lt_cnt po) 
+  next stk' po'
+  (Heq: find_next_visit_in_stk succs visited po stk = inl (next, stk', po')),
+  a2p_lt_cnt po'.
+Proof.
+  induction stk as [|[fr todo] stk]; simpl; intros.
+    congruence.
+
+    inv_mbind_app.
+    Case "push".
+      destruct_let. uniq_result. auto.
+    Case "pop".
+      apply IHstk in Heq; auto using a2p_lt_cnt__postorder_inc.
+Qed.
+
+Lemma find_next_visit_in_stk__wf_order: forall succs stk visited
+  po (Hwf: wf_order po) next stk' po'
+  (Heq: find_next_visit_in_stk succs visited po stk = inl (next, stk', po')),
+  wf_order po'.
+Proof.
+  intros.
+  destruct Hwf as [J1 J2]. 
+  unfold wf_order.
+  eapply find_next_visit_in_stk__a2p_injective in J2; eauto.
+  eapply find_next_visit_in_stk__a2p_lt_cnt in J1; eauto.
+Qed.
+
+Lemma wf_order__find_next_visit_in_stk_inr__wf_order: forall succs 
+  stk visited po1 (Hwf : wf_order po1) po2 
+  (Heq: find_next_visit_in_stk succs visited po1 stk = inr po2),
+  wf_order po2.
+Proof.
+  unfold wf_order.
+  induction stk as [|[fr todo] stk]; simpl; intros.
+    uniq_result. tauto.
+
+    inv_mbind_app.
+      destruct_let. congruence.
+
+      destruct Hwf as [Hwf1 Hwf2].
+      apply IHstk in Heq; auto using a2p_injective__postorder_inc,
+                                     a2p_lt_cnt__postorder_inc.
+Qed.
+
+Lemma entry_wf_order: forall pinit,
+  wf_order
+    {| PO_cnt := pinit; PO_a2p := ATree.empty positive |}.
+Proof.
+  intros.
+  split.
+    intros p a Hget. rewrite ATree.gempty in Hget. congruence.
+    intros p a1 a2 Hget1 Hget2. rewrite ATree.gempty in Hget1. congruence.
+Qed.
+
+Lemma dfs_wf: forall scs entry pinit po 
+  (Hdfs: dfs scs entry pinit = po), wf_order po.
+Proof.
+  intros.
+  eapply Inv.dfs_wf with 
+    (wf_stack:=fun scs v po stk=>wf_order po)
+    (wf_po:=fun scs po=>wf_order po) in Hdfs; 
+    eauto using wf_order__find_next_visit_in_stk_inr__wf_order,
+                find_next_visit_in_stk__wf_order, entry_wf_order.
+Qed.
+
+Lemma dfs_inj: forall scs entry pinit po 
+  (Hdfs: dfs scs entry pinit = po) (p:positive) a1 a2
+  (Hget2 : (PO_a2p po) ! a2 = Some p) (Hget1 : (PO_a2p po) ! a1 = Some p),
+  a1 = a2.
+Proof.
+  intros.
+  apply dfs_wf in Hdfs.
+  destruct Hdfs as [_ J].
+  eapply J; eauto.
+Qed.
+
+End Injective. 
 
